RiseDecoupled.v
@@ -4,7 +4,7 @@ Require Import List.
 Import ListNotations.
 Open Scope list_scope.
 
-
+Require Import Omega.
 
 Require Import PeanoNat.
 
@@ -13,6 +13,8 @@ Existing Instance latch_eq_dec.
 
 Require Import Coq.Logic.FunctionalExtensionality.
 Import Coq.Logic.ProofIrrelevance.
+Require Import Coq.Program.Equality.
+
 
 
 Section RiseDecoupled.
@@ -108,6 +110,12 @@ Section RiseDecoupled.
                          | _ => 0
                          end
    |}.
+
+About input_RD.
+Lemma rd_triples : forall e1 p e2,
+      In (e1, p, e2) (mg_triples rise_decoupled) <->
+      e1 = input_RD p /\ e2 = output_RD p.
+Admitted.
 
 
 
@@ -234,28 +242,332 @@ Qed.
 
 
 
+  Ltac simplify_in_FE :=
+      repeat match goal with
+      | [ H : In ?x (output_event rise_decoupled) |- _ ] => eapply in_output_event in H; eauto;
+                                                            destruct H as [? H]
+      | [ H : In ?x (input_event rise_decoupled) |- _ ] => eapply in_input_event in H; eauto;
+                                                            destruct H as [? H]
+      | [ H : In ?x (mg_triples rise_decoupled) |- _ ] => apply rd_triples in H; destruct H; subst; simpl in *
+      | [ |- In (?p, _) (output_event rise_decoupled) ] => eapply in_output_event; eauto;
+                                                           exists (input_RD p)
+      | [ |- In (_,?p) (input_event rise_decoupled) ] => eapply in_input_event; eauto;
+                                                           exists (output_RD p)
+      | [ |- In (_,_,_) (mg_triples rise_decoupled) ] => apply rd_triples; split; auto
+      end.
+
+  Ltac compare_in x l := 
+    let H := fresh "Heq" in
+    destruct (in_dec' x l) as [H | ?];
+    simplify_in_FE;
+      try match goal with
+      | [ H : Fall _ = Rise _ |- _ ] => inversion H 
+      | [ H : Fall (Even _) = Fall (Odd _) |- _ ] => inversion H
+      | [ H : Fall (Odd _) = Fall (Even _) |- _ ] => inversion H
+      | [ H : Rise _ = Fall _ |- _ ] => inversion H
+      | [ H : Rise (Even _) = Rise (Odd _) |- _ ] => inversion H
+      | [ H : Rise (Odd _) = Rise (Even _) |- _ ] => inversion H
+      end.
+
+  Ltac compare_next :=
+    match goal with
+    | [ |- context[ in_dec' ?x ?l ] ] => compare_in x l
+    | [ H : context[ in_dec' ?x ?l ] |- _ ] => compare_in x l
+    end;
+    repeat match goal with
+      | [ H : ~ In (_, _) (output_event rise_decoupled) |- _ ] => contradict H; simplify_in_FE; fail
+      | [ H : ~ In (_, _) (input_event rise_decoupled) |- _ ] => contradict H; simplify_in_FE; fail
+    end.
+
+
+
+Ltac specialize_enabled_constraints :=
+  repeat match goal with
+  | [ HEO : In (_,_) (even_odd_neighbors c)
+    , H : forall x, In _ (even_odd_neighbors c) -> _
+    |- _] => specialize (H _ HEO)
+  | [ HEO : In (_,_) (even_odd_neighbors c)
+    , H : forall x y, In _ (even_odd_neighbors c) -> _
+    |- _] => specialize (H _ _ HEO)
+  | [ HOE : In (_,_) (odd_even_neighbors c)
+    , H : forall x, In _ (odd_even_neighbors c) -> _
+    |- _] => specialize (H _ HOE)
+  | [ HOE : In (_,_) (odd_even_neighbors c)
+    , H : forall x y, In _ (odd_even_neighbors c) -> _
+    |- _] => specialize (H _ _ HOE)
+  end.
+
+Ltac get_enabled_constraints :=
+  try match goal with
+  | [ H : is_enabled rise_decoupled _ _ |- _ ] => apply is_enabled_RD_equiv in H; inversion H; subst
+  end; specialize_enabled_constraints.
+
+
+
+Lemma rd_loop_eo : forall t m,
+    {rise_decoupled}⊢ t ↓ m ->
+    forall E O, In (E,O) (even_odd_neighbors c) ->
+        m (Even_fall E) + m (Even_odd_fall E O) + m (Odd_even_rise E O) = 1.
+Proof.
+  intros t m Hm.
+  induction Hm; intros E O pfEO.
+  + reflexivity.
+  + subst. unfold fire.
+    repeat compare_next;
+      get_enabled_constraints; omega.
+Qed.
+
+Lemma rd_loop_odd : forall t m,
+    {rise_decoupled}⊢ t ↓ m ->
+    forall E O, In (E,O) (even_odd_neighbors c) ->
+    m (Odd_fall O) + m (Odd_rise O) = 1.
+Proof.
+  intros t m Hm.
+  induction Hm; intros E O pfEO.
+  + reflexivity.
+  + subst. unfold fire.
+    repeat compare_next; get_enabled_constraints; omega.
+Qed.
+
+Lemma rd_loop_oe : forall t m,
+    {rise_decoupled}⊢ t ↓ m ->
+    forall O E, In (O,E) (odd_even_neighbors c) ->
+        m (Odd_fall O) + m (Odd_even_fall O E) + m (Even_odd_rise O E) = 1.
+Proof.
+  intros t m Hm.
+  induction Hm; intros O E pfOE.
+  + reflexivity.
+  + subst. unfold fire.
+    repeat compare_next;
+      get_enabled_constraints; omega.
+Qed.
+
+Lemma rd_loop_even : forall t m,
+    {rise_decoupled}⊢ t ↓ m ->
+    forall O E, In (O,E) (odd_even_neighbors c) ->
+    m (Even_fall E) + m (Even_rise E) = 1.
+Proof.
+  intros t m Hm.
+  induction Hm; intros O E pfOE.
+  + reflexivity.
+  + subst. unfold fire.
+    repeat compare_next; get_enabled_constraints; omega.
+Qed.
+
+Lemma enabled_input_0 : forall t m,
+    {rise_decoupled}⊢ t ↓ m ->
+    forall p, is_enabled_RD (input_RD p) m ->
+    (forall p' : transitions_RD, m p' = 0 \/ m p' = 1) ->
+    m p = 0.
+Proof.
+  intros t m Hm. induction Hm; intros p Henabled IH.
+  + admit.
+  + subst. unfold fire.
+    compare_next. admit (*?*).
+    compare_next. admit.
+Abort.
+
+
+Lemma rd_safe : forall t m,
+    {rise_decoupled}⊢ t ↓ m ->
+    forall p, m(p) = 0 \/ m(p) = 1.
+Proof.
+  intros t m Hm.
+  induction Hm; intros p.
+  * destruct p; simpl; auto.
+  * apply is_enabled_RD_equiv in H.
+    subst.
+    unfold fire.
+    compare_next.
+    { destruct (IHHm p) as [Hp | Hp]; rewrite Hp; auto. }
+    compare_next.
+    { destruct (IHHm p) as [Hp | Hp]; rewrite Hp; auto.
+      contradict Hp. (* based on the fact that (input_RD p) is enabled in m *) admit.
+    }
+    { apply IHHm. }
+Abort.
 
 
 Lemma fall_enabled_even_opaque : forall s m O E,
     {rise_decoupled}⊢ s ↓ m ->
-    is_enabled rise_decoupled (Fall (Odd O)) m ->
+(*    is_enabled rise_decoupled (Fall (Odd O)) m -> *)
+    0 < m (Even_odd_fall E O) ->
     In (E,O) (even_odd_neighbors c) ->
     transparent s (Even E) = false.
-Admitted.
+Proof.
+  intros t; induction t as [P | e t]; intros m O E Hm Henabled Hneighbor.
+  * simpl in *.
+    inversion Hm; subst.
 
-Lemma fall_enabled_odd_opaque : forall s m O E,
-    {rise_decoupled}⊢ s ↓ m ->
-    is_enabled rise_decoupled (Fall (Even E)) m ->
+    apply H0.
+    apply RD_is_enabled_equiv.
+    constructor; intros O' HO'; auto.
+
+  * simpl.
+    inversion Hm; subst.
+    unfold fire in Henabled.
+    assert (Rise (Even E) <> e).
+    { inversion 1; subst. 
+      repeat get_enabled_constraints.
+      (* if it were, then (E+) is enabled, meaning that m0(O- -> E+) = 1, which further means that
+        m0(E+ -> E-) = 0 and m0(E- -> O-) = 0. *)
+      unfold fire in *.
+      repeat compare_next.
+      set (loop := rd_loop_eo _ _ H4 _ _ Hneighbor).
+      omega.
+    }
+    reduce_eqb.
+    compare (Fall (Even E) : event even odd) e; auto.
+    (* e is enabled in m0=t. e <> E+, e <> E-. *)
+    (* Since O- is enabled in (e::t), e must be equal to O+. *)
+
+    repeat compare_next; find_contradiction.
+    { contradict Henabled. 
+      set (Hloop := rd_loop_eo _ _ H4 _ _ Hneighbor).
+      omega.
+      (* since m0(E- → O-) = 0 or 1, it cannot be the case that 0 < m0(E- → O-)-1 *)
+    }
+    { eapply IHt; eauto. }
+Qed.
+
+Lemma fall_enabled_odd_opaque : forall t m O E,
+    {rise_decoupled}⊢ t ↓ m ->
+    0 < m (Odd_even_fall O E) ->
+(*    is_enabled rise_decoupled (Fall (Even E)) m ->*)
     In (O,E) (odd_even_neighbors c) ->
-    transparent s (Odd O) = false.
+    transparent t (Odd O) = false.
+Proof.
+  intros t; induction t as [P | e t]; intros m O E Hm Henabled Hneighbor.
+
+  * simpl in *.
+    inversion Hm; subst.
+    (* I think the precondition of H0 is not enough to know that P(Odd O) = false, since neither O+ nor O- are enabled in the initial state. *)
+(*    apply H0.*)
+    admit.
+
+  * simpl.
+    inversion Hm; subst.
+    unfold fire in Henabled.
+    assert (Rise (Odd O) <> e).
+    { inversion 1; subst. 
+      repeat get_enabled_constraints.
+      unfold fire in *.
+      repeat compare_next.
+      set (loop := rd_loop_oe _ _ H4 _ _ Hneighbor).
+      omega.
+    }
+    reduce_eqb.
+    compare (Fall (Odd O) : event even odd) e; auto.
+    (* e is enabled in m0=t. e <> O+, e <> O-. *)
+    (* Since E- is enabled in (e::t), e must be equal to E+. *)
+
+    repeat compare_next; find_contradiction.
+    { contradict Henabled. 
+      set (Hloop := rd_loop_oe _ _ H4 _ _ Hneighbor).
+      omega.
+    }
+    { eapply IHt; eauto. }
 Admitted.
 
-Lemma fall_enabled_even_odd : forall s m O E,
+Lemma fall_enabled_even_odd_strong : forall s m O E,
     {rise_decoupled}⊢ s ↓ m ->
+(*    is_enabled rise_decoupled (Fall (Odd O)) m -> *)
+    In (E,O) (even_odd_neighbors c) ->
+     (0 < m (Even_odd_fall E O) -> num_events (Fall (Even E)) s = 1 + num_events (Fall (Odd O)) s)
+  /\ (0 < m (Odd_even_rise E O) -> num_events (Fall (Even E)) s = num_events (Fall (Odd O)) s)
+  /\ (0 < m (Even_fall E) -> num_events (Fall (Even E)) s = num_events (Fall (Odd O)) s).
+Proof.
+  intros t; induction t as [P | e t]; intros m O E Hm  Hneighbor; repeat split; intros Henabled.
+
+  * inversion Hm; subst.
+    simpl in Henabled.
+    find_contradiction.
+
+
+  * inversion Hm; subst.
+    unfold fire in Henabled.
+    simpl.
+    compare (Fall (Even E) : event even odd) e; simpl; reduce_eqb.
+    { specialize (IHt _ _ _ H4 Hneighbor).
+      destruct IHt as [IH1 [IH2 IH3]].
+      rewrite IH3; auto.
+      get_enabled_constraints; auto.
+    }
+    compare (Fall (Odd O) : event even odd) e; simpl; reduce_eqb.
+    { repeat compare_next; reduce_eqb.
+      contradict Henabled.
+      set (Hloop := rd_loop_eo _ _ H4 _ _ Hneighbor).
+      omega.
+    }
+    repeat compare_next; reduce_eqb.
+    { specialize (IHt _ _ _ H4 Hneighbor).
+      destruct IHt as [IH1 [IH2 IH3]].
+      apply IH1; auto.
+    }
+
+
+  * inversion Hm; subst.
+    unfold fire in Henabled.
+    specialize (IHt _ _ _ H4 Hneighbor).
+    destruct IHt as [IH1 [IH2 IH3]].
+    set (Hloop := rd_loop_eo _ _ H4 _ _ Hneighbor).
+    simpl.
+    compare (Fall (Even E) : event even odd) e; simpl; reduce_eqb.
+    { repeat compare_next; reduce_eqb. 
+      get_enabled_constraints.
+      contradict Henabled.
+      omega.
+    }
+    compare (Fall (Odd O) : event even odd) e; simpl; reduce_eqb.
+    { repeat compare_next.
+      get_enabled_constraints.
+      apply IH1; auto.
+    }
+    repeat compare_next; find_contradiction.
+    { contradict Henabled.
+      omega.
+    }
+    { apply IH2; auto. }
+
+  * inversion Hm; subst.
+    unfold fire in Henabled.
+    specialize (IHt _ _ _ H4 Hneighbor).
+    destruct IHt as [IH1 [IH2 IH3]].
+    set (Hloop := rd_loop_eo _ _ H4 _ _ Hneighbor).
+
+    simpl.
+    compare (Fall (Even E) : event even odd) e; simpl; reduce_eqb.
+    { repeat compare_next; reduce_eqb.
+      get_enabled_constraints.
+      contradict Henabled.
+      omega.
+    }
+    compare (Fall (Odd O) : event even odd) e; simpl; reduce_eqb.
+    { repeat compare_next.
+      get_enabled_constraints.
+      contradict Henabled.
+      omega.
+    }
+    repeat compare_next; find_contradiction.
+    { get_enabled_constraints.
+      apply IH2; auto.
+    }
+    { apply IH3; auto. }
+Qed.
+
+Lemma fall_enabled_even_odd : forall t m O E,
+    {rise_decoupled}⊢ t ↓ m ->
     is_enabled rise_decoupled (Fall (Odd O)) m ->
     In (E,O) (even_odd_neighbors c) ->
-    num_events (Fall (Even E)) s = 1 + num_events (Fall (Odd O)) s.
-Admitted.
+    num_events (Fall (Even E)) t = 1 + num_events (Fall (Odd O)) t.
+Proof.
+  intros t m O E Hm Henabled Hneighbors.
+  set (H := fall_enabled_even_odd_strong t m O E Hm Hneighbors).
+  destruct H as [H1 [H2 H3]].
+  apply H1.
+  get_enabled_constraints; auto.
+Qed.
+
 
 Lemma fall_enabled_odd_even : forall s m O E,
     {rise_decoupled}⊢ s ↓ m ->
@@ -267,24 +579,19 @@ Admitted.
 
 
 
-Require Import Coq.Program.Equality.
-Lemma rel_fe : forall l b t v,
-    async_rel c init_st l b t v ->
-    b = false ->
-    forall m,
-    {rise_decoupled}⊢ t ↓ m ->
-    v = sync_eval c init_st (num_events (Fall l) t) l.
+Theorem rise_decoupled_flow_equivalence_rel : flow_equivalence_rel _ _ rise_decoupled c init_st.
 Proof.
-  intros l b t v Hrel.
-  
-  induction Hrel; intros Hb m Hm; find_contradiction.
+  intros l t v Hrel.
+  dependent induction Hrel; intros [m Hm].
   * destruct l as [O | E].
     (* l must be odd *)
-    2:{ contradict H. inversion Hm as [P' Htransparent Hopaque | ].
-        rewrite Hopaque; [inversion 1 | ].
-        apply RD_is_enabled_equiv.
-        simpl.
-        constructor; intros; auto.
+    2:{ assert (P (Even E) = true).
+        { inversion Hm as [P' Htransparent Hopaque | ].
+          rewrite Hopaque; [auto | ].
+          apply RD_is_enabled_equiv.
+          constructor; intros; auto.
+        }
+        find_contradiction.
     }
     simpl. reflexivity.
   * inversion Hm as [ | e0 m0 ? t' Henabled Hfire Hm']; subst; rename m0 into m.
@@ -294,26 +601,19 @@ Proof.
 
   * inversion Hm as [ | e0 m0 ? t' Henabled Hfire Hm']; subst; rename m0 into m.
     simpl in *.
-    reduce_eqb.
-    set (st' := fun n => fun l' => match l with
-                          | Even _ => sync_eval c init_st n l'
-                          | Odd _  => sync_eval c init_st (S n) l'
-                          end).
-    assert (Hstep : forall n, sync_eval c init_st (S n) l = next_state c (st' n) l).
-    { destruct l; intros n; simpl.
-      + apply f_equal. apply functional_extensionality. intros [E HE]. simpl.
-        unfold even_state. simpl. reflexivity.
-      + apply f_equal. apply functional_extensionality. intros [O HO]. simpl.
-        unfold even_state. simpl. reflexivity.
-    }
-    rewrite Hstep.
-    apply next_state_eq.
+    reduce_eqb. Search sync_eval S.
+    erewrite sync_eval_S; eauto.
     intros l' Hl'.
-    unfold st'.
     erewrite H1; eauto.
     2:{ inversion Hl'; subst. 
-        { eapply fall_enabled_even_opaque; eauto. }
-        { eapply fall_enabled_odd_opaque; eauto. }
+        { eapply fall_enabled_even_opaque; eauto. 
+          get_enabled_constraints.
+          auto.
+        }
+        { eapply fall_enabled_odd_opaque; eauto.
+          get_enabled_constraints.
+          auto.
+        }
     }
 
     { inversion Hl'; subst.
@@ -323,7 +623,7 @@ Proof.
         
   Qed.
 
-
+(*
 
   Lemma fall_enabled_transparent : forall (t : trace even odd)
                                           (m : marking transitions_RD),
@@ -493,5 +793,6 @@ Abort.
       2:{ apply Hopaque. }
       reflexivity.
   Qed.
+*)
 
 End RiseDecoupled.
